\documentclass{minimal}


\begin{document}

\[
P(fila, columna, signo, turno)
\]


fila = 3

columna = 3

signo = 3

turno = 2

P = 54

letras chr(256) -- chr(310)

tseitin regla Edgar chr(400) -- chr(899)

tseitin regla Nicolas chr(900) -- chr(1399)

tseitin regla Juan Luis chr(1400) -- chr(1899)


$\beta$ codifica que no hay cambio


\[
\beta(x,y,z) \leftrightarrow ( P(x,y,z,0) \to P(x,y,z,1)  )
\]

\[
\bigwedge\left(   ( P(x,y,E,0) \wedge P(x,y,O,1)  ) \leftrightarrow (\bigvee( \beta(x',y',z)  ) )    \right)
\]

\textbf{Regla - Ganar cuando es posible}
\[A \leftrightarrow \bigwedge\left(P(x,y,O,0)\wedge P(x+1,y,O,0) \rightarrow P(x+2,y,O,1)\right)\]
\[B \leftrightarrow \bigwedge\left(P(x,y,O,0)\wedge P(x,y+1,O,0) \rightarrow P(x,y+2,O,1)\right)\]
\[C \leftrightarrow \bigwedge\left(P(a,a,O,0)\wedge P(a+1,a+1,O,0) \rightarrow P(a+2,a+2,O,1)\right)\]
\[D \leftrightarrow \bigwedge\left(P(x,y,O,0)\wedge P(x-1,y+1,O,0) \rightarrow P(x-2,y+2,O,1)\right), x+y=2\]
\[A\wedge B\wedge C\wedge D\]


\textbf{Regla - No perder}

%$$E \leftrightarrow  \bigwedge_{c\,{\in}\,\mbox{\textsc{columna}}} \left(\left(\left(P(0,c,O,0) \wedge P(1,c,O,0) \right) \rightarrow P(2,c,X,1)\right) \wedge \left(\left( P(1,c,O,0) \wedge P(2,c,O,0) \right) \rightarrow P(0,c,X,1) \right) \wedge $$
%$$\left(\left(P(0,c,O,0) \wedge P(2,c,O,0)\right) \rightarrow P(1,c,X,1)\right)\right)\right)$$

$$E \leftrightarrow  \left(\bigwedge_{c\,{\in}\,\mbox{\textsc{columna}}} \left( \bigwedge_{f\,{\in}\,\mbox{\textsc{fila}}} \left(\bigwedge_{\alpha \,{\in}\,\mbox{\textsc{fila}}- \{f\}} P(\alpha,c,O,0) \right) \rightarrow P(f,c,X,1)\right)\right) $$

$$F \leftrightarrow  \left(\bigwedge_{f\,{\in}\,\mbox{\textsc{fila}}} \left( \bigwedge_{c\,{\in}\,\mbox{\textsc{columna}}} \left(\bigwedge_{\alpha \,{\in}\,\mbox{\textsc{columna}}- \{c\}} P(f,\alpha,O,0) \right) \rightarrow P(f,c,X,1)\right)\right) $$

%//$$F \leftrightarrow  \bigwedge_{f\,{\in}\,\mbox{\textsc{fila}}} \left(\left(\left(P(f,0,O,0) \wedge P(f,1,O,0) \right) \rightarrow P(f,2,X,1)\right) \wedge \left(\left( P(f,1,O,0) \wedge P(f,2,O,0) \right) \rightarrow P(f,0,X,1) \right) \wedge $$//
%$$\left(\left(P(f,0,O,0) \wedge P(f,2,O,0)\right) \rightarrow P(f,1,X,1)\right)\right)\right)$$

$$G \leftrightarrow \left( \bigwedge_{\alpha \,{\in}\,\mbox{\textsc{columna}}} \left(\bigwedge_{\beta \,{\in}\,\mbox{\textsc{columna}}- \{\alpha\}} P(\beta,\beta,O,0) \right) \rightarrow P(\alpha,\alpha,X,1)\right) $$

$$H \leftrightarrow \left( \bigwedge_{\alpha \,{\in}\,\mbox{\textsc{columna}}} \left(\bigwedge_{\beta \,{\in}\,\mbox{\textsc{columna}}- \{\alpha\}} P(\beta,2 - \beta,O,0) \right) \rightarrow P(\alpha,2 - \alpha,X,1)\right) $$
\[E\wedge F\wedge G\wedge H\]
\end{document}
